Getting rid of UVALUE_Load and remaining MEMORYSTATE stuff...

src/coq/Semantics/DynamicValues.v
@@ -180,9 +180,6 @@ Definition ll_float  := Floats.float32.
 Definition ll_double := Floats.float.
 
 Module DVALUE(A:Vellvm.Semantics.MemoryAddress.ADDRESS).
-  Variable memory : Type.
-  Context {RDM:RelDec (@eq memory)} {RDMC:RelDec_Correct RDM}.
-
   (* The set of dynamic values manipulated by an LLVM program. *)
  Unset Elimination Schemes.
 Inductive dvalue : Set :=
@@ -284,7 +281,6 @@ Inductive uvalue : Type :=
    id". *)
 | UVALUE_ExtractByte      (uv : uvalue) (dt : dtyp) (idx : uvalue) (sid : store_id)
 | UVALUE_ConcatBytes      (uvs : list uvalue) (dt : dtyp)
-| UVALUE_Load             (t:dtyp) (a:uvalue) (m:memory)
 .
 Set Elimination Schemes.
 
@@ -319,7 +315,6 @@ Section UvalueInd.
   Hypothesis IH_Select         : forall (cnd:uvalue) (v1:uvalue) (v2:uvalue), P cnd -> P v1 -> P v2 -> P (UVALUE_Select cnd v1 v2).
   Hypothesis IH_ExtractByte : forall (uv : uvalue) (dt : dtyp) (idx : uvalue) (sid : N), P uv -> P idx -> P (UVALUE_ExtractByte uv dt idx sid).
   Hypothesis IH_ConcatBytes : forall (dt : dtyp) (uvs : list uvalue), (forall u, In u uvs -> P u) -> P (UVALUE_ConcatBytes uvs dt).
-  Hypothesis IH_Load : forall (dt : dtyp) (ua : uvalue) (m : memory), P ua -> P (UVALUE_Load dt ua m).
 
   Lemma uvalue_ind : forall (uv:uvalue), P uv.
     fix IH 1.
@@ -367,8 +362,6 @@ Section UvalueInd.
         fix IHuvs 1. intros [|u uvs']. intros. inversion H.
         intros u' [<-|Hin]. apply IH. eapply IHuvs. apply Hin.
       }
-    - apply IH_Load.
-      apply IH.
   Qed.
 End UvalueInd.
 
@@ -764,7 +757,6 @@ Section DecidableEquality.
               | UVALUE_Select u v t, UVALUE_Select u' v' t' => _
               | UVALUE_ExtractByte uv dt idx sid, UVALUE_ExtractByte uv' dt' idx' sid' => _
               | UVALUE_ConcatBytes uvs dt, UVALUE_ConcatBytes uvs' dt' => _
-              | UVALUE_Load dt ua m, UVALUE_Load dt' ua' m' => _
               | _, _ => _
               end); try (ltac:(dec_dvalue); fail).
     - destruct (A.eq_dec a1 a2)...
@@ -821,13 +813,10 @@ Section DecidableEquality.
       destruct (dtyp_eq_dec dt dt')...
     - destruct (lsteq_dec uvs uvs')...
       destruct (dtyp_eq_dec dt dt')...
-    - destruct (f ua ua')...
-      destruct (dtyp_eq_dec dt dt')...
-      destruct (rel_dec_p m m')...
   Qed.
 
   
-  #[global] Instance eq_dec_uvalue `{RD: RelDec memory}: RelDec (@eq uvalue) := RelDec_from_dec (@eq uvalue) (@uvalue_eq_dec).
+  #[global] Instance eq_dec_uvalue : RelDec (@eq uvalue) := RelDec_from_dec (@eq uvalue) (@uvalue_eq_dec).
   #[global] Instance eqv_uvalue : Eqv (uvalue) := (@eq uvalue).
   Hint Unfold eqv_uvalue : core.
   #[global] Instance eq_dec_uvalue_correct: @RelDec.RelDec_Correct uvalue (@Logic.eq uvalue) _ := _.
