src/coq/Handlers/Serialization.v
@@ -419,8 +419,7 @@ Module Make(Addr:MemoryAddress.ADDRESS)(LLVMIO: LLVM_INTERACTIONS(Addr))(SIZEOF:
        | UVALUE_ShuffleVector _ _ _
        | UVALUE_ExtractValue _ _
        | UVALUE_InsertValue _ _ _
-       | UVALUE_Select _ _ _
-       | UVALUE_Load _ _ _ =>
+       | UVALUE_Select _ _ _ =>
          sid <- fresh_sid;;
          ret (to_ubytes uv dt sid)
 
@@ -1017,8 +1016,6 @@ Module Make(Addr:MemoryAddress.ADDRESS)(LLVMIO: LLVM_INTERACTIONS(Addr))(SIZEOF:
         | UVALUE_ExtractByte byte dt idx sid =>
           (* TODO: maybe this is just an error? ExtractByte should be guarded by ConcatBytes? *)
           lift (failwith "Attempting to concretize UVALUE_ExtractByte, should not happen.")
-        | UVALUE_Load dt uv mem =>
-          UVALUE_Load dt
 
         | _ => (lift (failwith "Attempting to convert a partially non-reduced uvalue to dvalue. Should not happen"))
 
